Prove of lemma_pred_4_1_b

src/dvspec/dafny/att_spec_proofs/ind_inv.dfy
@@ -1,4 +1,5 @@
 include "../commons.dfy"
+include "../att_spec_proofs/helper_sets_lemmas.dfy"
 include "../specification/dvc_spec.dfy"
 include "../specification/consensus.dfy"
 include "../specification/network.dfy"
@@ -14,6 +15,7 @@ module Att_Ind_Inv_With_Empty_Initial_Attestation_Slashing_DB
     import opened DVCNode_Spec
     import opened DV    
     import opened Att_Inv_With_Empty_Initial_Attestation_Slashing_DB
+    import opened Helper_Sets_Lemmas
 
     lemma ConsensusSpec_Init_implies_inv41<D(!new, 0)>(dvn: DVState, ci: ConsensusInstance<D>)
     requires ConsensusSpec.Init(ci, dvn.all_nodes, dvn.honest_nodes_states.Keys)
@@ -83,4 +85,523 @@ module Att_Ind_Inv_With_Empty_Initial_Attestation_Slashing_DB
     lemma DV_Init_implies_thresholds(dvn: DVState)
     requires DV.Init(dvn, {})
     ensures |dvn.honest_nodes_states.Keys| >= |dvn.all_nodes| - f(|dvn.all_nodes|) 
+
+    lemma lemma_pred_4_1_b_helper(
+        s: DVState,
+        event: DV.Event,
+        s': DVState
+    )
+    // requires NextEvent(s, event, s')
+    requires pred_4_1_b(s)
+    requires s'.all_nodes == s.all_nodes;
+    requires s'.honest_nodes_states.Keys == s.honest_nodes_states.Keys;
+    requires forall n | n in s'.honest_nodes_states.Keys :: s.honest_nodes_states[n].bn.attestations_submitted == s'.honest_nodes_states[n].bn.attestations_submitted;
+    requires s.att_network.allMessagesSent <= s'.att_network.allMessagesSent;    
+    ensures pred_4_1_b(s');
+    {
+            forall hn, a |
+                && hn in s.honest_nodes_states.Keys 
+                && a in s.honest_nodes_states[hn].bn.attestations_submitted
+            ensures exists hn', att_share: AttestationShare, fork_version :: pred_4_1_b_exists(s', hn', att_share, fork_version, a);
+            {
+                var hn', att_share: AttestationShare, fork_version :|
+                    pred_4_1_b_exists(s, hn', att_share, fork_version, a);
+                
+                assert pred_4_1_b_exists(s', hn', att_share, fork_version, a);
+                assert exists hn', att_share: AttestationShare, fork_version :: pred_4_1_b_exists(s', hn', att_share, fork_version, a);
+            }
+            assert pred_4_1_b(s');
+    }
+
+    // lemma lemma_pred_4_1_b_f_start_next_duty()
+    // ensures  
+    //         forall
+    //             s: DVCNodeState,
+    //             attestation_duty: AttestationDuty,
+    //             s': DVCNodeState
+    //         |
+    //             && f_start_next_duty.requires(s, attestation_duty)
+    //             && s' == f_start_next_duty(s, attestation_duty).state
+    //         ::
+    //             s'.bn.attestations_submitted == s.bn.attestations_submitted
+    // {
+
+    // }
+
+    lemma lemma_pred_4_1_b_f_serve_attestation_duty(
+        s: DVCNodeState,
+        attestation_duty: AttestationDuty,
+        s': DVCNodeState
+    )  
+    requires f_serve_attestation_duty.requires(s, attestation_duty)
+    requires s' == f_serve_attestation_duty(s, attestation_duty).state
+    ensures s'.bn.attestations_submitted == s.bn.attestations_submitted      
+    {
+        var s_mod := s.(
+                attestation_duties_queue := s.attestation_duties_queue + [attestation_duty],
+                all_rcvd_duties := s.all_rcvd_duties + {attestation_duty}
+            );
+        lemma_pred_4_1_b_f_check_for_next_queued_duty(s_mod, s');
+    }
+
+    lemma lemma_pred_4_1_b_f_check_for_next_queued_duty(
+        s: DVCNodeState,
+        s': DVCNodeState
+    )
+    requires f_check_for_next_queued_duty.requires(s)
+    requires s' == f_check_for_next_queued_duty(s).state
+    ensures s'.bn.attestations_submitted == s.bn.attestations_submitted
+    decreases s.attestation_duties_queue
+    {
+        if  && s.attestation_duties_queue != [] 
+            && (
+                || s.attestation_duties_queue[0].slot in s.future_att_consensus_instances_already_decided
+                || !s.current_attestation_duty.isPresent()
+            )    
+        {
+            
+                if s.attestation_duties_queue[0].slot in s.future_att_consensus_instances_already_decided.Keys 
+                {
+                    var queue_head := s.attestation_duties_queue[0];
+                    var new_attestation_slashing_db := f_update_attestation_slashing_db(s.attestation_slashing_db, s.future_att_consensus_instances_already_decided[queue_head.slot]);
+                    var s_mod := s.(
+                        attestation_duties_queue := s.attestation_duties_queue[1..],
+                        future_att_consensus_instances_already_decided := s.future_att_consensus_instances_already_decided - {queue_head.slot},
+                        attestation_slashing_db := new_attestation_slashing_db,
+                        attestation_consensus_engine_state := updateConsensusInstanceValidityCheck(
+                            s.attestation_consensus_engine_state,
+                            new_attestation_slashing_db
+                        )                        
+                    );
+                    lemma_pred_4_1_b_f_check_for_next_queued_duty(s_mod, s');
+                }
+                else
+                {
+                    // var new_process := s.(
+                    //     attestation_duties_queue := s.attestation_duties_queue[1..]
+                    // );         
+                    // lemma_pred_4_1_b_f_start_next_duty();
+                }
+
+        }
+    }
+
+    lemma lemma_pred_4_1_b_f_att_consensus_decided(
+        s: DVCNodeState,
+        id: Slot,
+        decided_attestation_data: AttestationData,        
+        s': DVCNodeState
+    )
+    requires f_att_consensus_decided.requires(s, id, decided_attestation_data)
+    requires s' == f_att_consensus_decided(s, id, decided_attestation_data).state
+    ensures s'.bn.attestations_submitted == s.bn.attestations_submitted
+    decreases s.attestation_duties_queue   
+    {
+        var local_current_attestation_duty := s.current_attestation_duty.safe_get();
+        var attestation_slashing_db := f_update_attestation_slashing_db(s.attestation_slashing_db, decided_attestation_data);
+
+        var fork_version := bn_get_fork_version(compute_start_slot_at_epoch(decided_attestation_data.target.epoch));
+        var attestation_signing_root := compute_attestation_signing_root(decided_attestation_data, fork_version);
+        var attestation_signature_share := rs_sign_attestation(decided_attestation_data, fork_version, attestation_signing_root, s.rs);
+        var attestation_with_signature_share := AttestationShare(
+                aggregation_bits := get_aggregation_bits(local_current_attestation_duty.validator_index),
+                data := decided_attestation_data, 
+                signature := attestation_signature_share
+            ); 
+
+        var s := 
+            s.(
+                current_attestation_duty := None,
+                attestation_shares_to_broadcast := s.attestation_shares_to_broadcast[local_current_attestation_duty.slot := attestation_with_signature_share],
+                attestation_slashing_db := attestation_slashing_db,
+                attestation_consensus_engine_state := updateConsensusInstanceValidityCheck(
+                    s.attestation_consensus_engine_state,
+                    attestation_slashing_db
+                )
+            );
+
+        lemma_pred_4_1_b_f_check_for_next_queued_duty(s, s');             
+    } 
+
+    lemma lemma_pred_4_1_b_f_listen_for_new_imported_blocks(
+        s: DVCNodeState,
+        block: BeaconBlock,
+        s': DVCNodeState
+    )
+    requires f_listen_for_new_imported_blocks.requires(s, block)
+    requires s' == f_listen_for_new_imported_blocks(s, block).state
+    ensures s'.bn.attestations_submitted == s.bn.attestations_submitted
+    {
+        var new_consensus_instances_already_decided := f_listen_for_new_imported_blocks_helper_1(s, block);
+
+        var att_consensus_instances_already_decided := s.future_att_consensus_instances_already_decided + new_consensus_instances_already_decided;
+
+        var future_att_consensus_instances_already_decided := 
+            f_listen_for_new_imported_blocks_helper_2(s, att_consensus_instances_already_decided);
+
+        var s :=
+                s.(
+                    future_att_consensus_instances_already_decided := future_att_consensus_instances_already_decided,
+                    attestation_consensus_engine_state := stopConsensusInstances(
+                                    s.attestation_consensus_engine_state,
+                                    att_consensus_instances_already_decided.Keys
+                    ),
+                    attestation_shares_to_broadcast := s.attestation_shares_to_broadcast - att_consensus_instances_already_decided.Keys,
+                    rcvd_attestation_shares := s.rcvd_attestation_shares - att_consensus_instances_already_decided.Keys                    
+                );                     
+
+        if s.current_attestation_duty.isPresent() && s.current_attestation_duty.safe_get().slot in att_consensus_instances_already_decided
+        {
+            // Stop(current_attestation_duty.safe_get().slot);
+            var decided_attestation_data := att_consensus_instances_already_decided[s.current_attestation_duty.safe_get().slot];
+            var new_attestation_slashing_db := f_update_attestation_slashing_db(s.attestation_slashing_db, decided_attestation_data);
+            var s := s.(
+                current_attestation_duty := None,
+                attestation_slashing_db := new_attestation_slashing_db,
+                attestation_consensus_engine_state := updateConsensusInstanceValidityCheck(
+                    s.attestation_consensus_engine_state,
+                    new_attestation_slashing_db
+                )                
+            );
+            assert s' == f_check_for_next_queued_duty(s).state;
+            lemma_pred_4_1_b_f_check_for_next_queued_duty(s, s');
+        }
+    }  
+
+    function recover_bls_signature(
+        r: Root,
+        signature: BLSSignature
+    ): BLSPubkey
+    requires exists pubkey :: verify_bls_siganture(r, signature, pubkey)
+    {
+        var pubkey :| verify_bls_siganture(r, signature, pubkey);
+        pubkey
+    }
+
+    lemma lemma_recover_bls_signature()
+    ensures forall r, s1, s2 |
+                && recover_bls_signature.requires(r, s1)
+                && recover_bls_signature.requires(r, s2)
+                && recover_bls_signature(r, s1) == recover_bls_signature(r, s2)
+            ::
+                s1 == s2
+    {
+        lemma_verify_bls_siganture();
+    }
+    
+
+    lemma lemma_pred_4_1_b_f_listen_for_attestation_shares(
+        process: DVCNodeState,
+        attestation_share: AttestationShare,
+
+        s': DVCNodeState,
+        dvn: DVState
+    )
+    requires f_listen_for_attestation_shares.requires(process, attestation_share)
+    requires s' == f_listen_for_attestation_shares(process, attestation_share).state
+    requires construct_signed_attestation_signature_assumptions_helper(
+        process.construct_signed_attestation_signature,
+        process.dv_pubkey,
+        dvn.all_nodes
+    )
+    requires dvn.honest_nodes_states.Keys <= dvn.all_nodes
+    requires var byz := dvn.all_nodes - dvn.honest_nodes_states.Keys; |byz| < f(|dvn.all_nodes|)
+    requires attestation_share in dvn.att_network.allMessagesSent
+    requires pred_rcvd_attestation_shares_is_in_all_messages_sent_single_node_state(dvn, process)
+    requires forall a | a in process.bn.attestations_submitted :: exists hn', att_share: AttestationShare, fork_version :: pred_4_1_b_exists(dvn, hn', att_share, fork_version, a)
+
+    ensures forall a | a in s'.bn.attestations_submitted :: exists hn', att_share: AttestationShare, fork_version :: pred_4_1_b_exists(dvn, hn', att_share, fork_version, a)
+    // ensures s'.bn.attestations_submitted == s.bn.attestations_submitted     
+    {
+        var activate_att_consensus_intances := process.attestation_consensus_engine_state.attestation_consensus_active_instances.Keys;
+
+        if 
+            || (activate_att_consensus_intances == {} && !process.latest_attestation_duty.isPresent())
+            || (activate_att_consensus_intances != {} && minSet(activate_att_consensus_intances) <= attestation_share.data.slot)
+            || (activate_att_consensus_intances == {} && process.current_attestation_duty.isPresent() && process.current_attestation_duty.safe_get().slot <= attestation_share.data.slot)                
+            || (activate_att_consensus_intances == {} && !process.current_attestation_duty.isPresent() && process.latest_attestation_duty.isPresent() && process.latest_attestation_duty.safe_get().slot < attestation_share.data.slot)
+            {
+                var k := (attestation_share.data, attestation_share.aggregation_bits);
+                var attestation_shares_db_at_slot := getOrDefault(process.rcvd_attestation_shares, attestation_share.data.slot, map[]);
+                
+                var new_attestation_shares_db := 
+                        process.rcvd_attestation_shares[
+                            attestation_share.data.slot := 
+                                attestation_shares_db_at_slot[
+                                            k := 
+                                                getOrDefault(attestation_shares_db_at_slot, k, {}) + 
+                                                {attestation_share}
+                                            ]
+                                ];
+
+                var process := process.(
+                    rcvd_attestation_shares := new_attestation_shares_db
+                );
+
+                            
+                if process.construct_signed_attestation_signature(process.rcvd_attestation_shares[attestation_share.data.slot][k]).isPresent()
+                {
+                    var aggregated_attestation := 
+                            Attestation(
+                                aggregation_bits := attestation_share.aggregation_bits,
+                                data := attestation_share.data,
+                                signature := process.construct_signed_attestation_signature(process.rcvd_attestation_shares[attestation_share.data.slot][k]).safe_get()
+                            );
+
+                    var att_shares := process.rcvd_attestation_shares[attestation_share.data.slot][k];
+                    assert construct_signed_attestation_signature_assumptions_helper_reverse(
+                        process.construct_signed_attestation_signature,
+                        process.dv_pubkey,
+                        dvn.all_nodes                    
+                    );
+
+                    assert process.construct_signed_attestation_signature(att_shares).isPresent();
+
+                    assert construct_signed_attestation_signature_assumptions_helper_reverse(
+                        process.construct_signed_attestation_signature,
+                        process.dv_pubkey,
+                        dvn.all_nodes
+                    );
+
+                    var data: AttestationData :|
+                        construct_signed_attestation_signature_assumptions_helper_reverse_helper(
+                            process.construct_signed_attestation_signature,
+                            process.dv_pubkey,
+                            dvn.all_nodes,
+                            att_shares,
+                            data                
+                        );
+
+                    assert pred_rcvd_attestation_shares_is_in_all_messages_sent_single_node_state(dvn, process);
+                    assert att_shares <= dvn.att_network.allMessagesSent;
+
+                    var fork_version := bn_get_fork_version(compute_start_slot_at_epoch(data.target.epoch));
+                    var signing_root := compute_attestation_signing_root(data, fork_version);
+ 
+
+                    var signers := 
+                    set signer, att_share | 
+                        && att_share in att_shares
+                        && signer in dvn.all_nodes
+                        && verify_bls_siganture(signing_root, att_share.signature, signer)
+                    ::
+                        signer;
+
+                    assert signers <= dvn.all_nodes;
+
+                    lemmaThereExistsAnHonestInQuorum(dvn.all_nodes, dvn.all_nodes - dvn.honest_nodes_states.Keys, signers);
+
+                    var h_s :| h_s in dvn.honest_nodes_states.Keys && h_s in signers;
+                    var h_s_att :| h_s_att in att_shares && verify_bls_siganture(signing_root, h_s_att.signature, h_s);
+
+                    // var attestation_signing_root := compute_attestation_signing_root(data, fork_version);
+
+                    // assert signing_root == attestation_signing_root;                    
+
+                    assert 
+                    && h_s in dvn.honest_nodes_states.Keys
+                    && h_s_att in dvn.att_network.allMessagesSent
+                    && h_s_att.data == data
+                    && verify_bls_siganture(signing_root, h_s_att.signature, h_s);
+
+                    assert 
+                    && h_s in dvn.honest_nodes_states.Keys
+                    && h_s_att in dvn.att_network.allMessagesSent
+                    && h_s_att.data == data
+                    // && var fork_version := bn_get_fork_version(compute_start_slot_at_epoch(data.target.epoch));
+                    && verify_bls_siganture(signing_root, h_s_att.signature, h_s);
+
+                    // assert pred_attestations_signature_by_honest_node_implies_existence_of_attestation_with_correct_data_helper(
+                    //     dvn,
+                    //     h_s_att,
+                    //     h_s,
+                    //     signing_root
+                    // );
+
+                    // var att_share' :| pred_attestations_signature_by_honest_node_implies_existence_of_attestation_with_correct_data_helper_helper(dvn, att_share', signing_root, h_s_att.signature);
+
+                    
+
+                    // assert verify_bls_siganture(attestation_signing_root, h_s_att.signature, h_s);
+
+                    assert pred_4_1_b_exists(
+                        dvn,
+                        h_s,
+                        h_s_att,
+                        fork_version,
+                        aggregated_attestation
+                    );
+
+                               
+                    
+                    var    state := process.(
+                            bn := process.bn.(
+                                attestations_submitted := process.bn.attestations_submitted + [aggregated_attestation]
+                            )
+                        );
+
+                    forall a | a in state.bn.attestations_submitted 
+                    {
+                        assert exists hn', att_share: AttestationShare, fork_version :: pred_4_1_b_exists(dvn, hn', att_share, fork_version, a);
+                    }
+                    assert s' == state;
+                }
+            }   
+    }
+
+
+    lemma lemma_pred_4_1_b(
+        s: DVState,
+        event: DV.Event,
+        s': DVState
+    )
+    requires NextEvent(s, event, s')
+    requires pred_4_1_b(s)
+    requires construct_signed_attestation_signature_assumptions_helper(
+        s.construct_signed_attestation_signature,
+        s.dv_pubkey,
+        s.all_nodes
+    )
+    requires forall n | n in s.honest_nodes_states.Keys :: s.honest_nodes_states[n].construct_signed_attestation_signature == s.construct_signed_attestation_signature
+    requires forall n | n in s.honest_nodes_states.Keys :: s.honest_nodes_states[n].dv_pubkey == s.dv_pubkey    
+    requires s.honest_nodes_states.Keys <= s.all_nodes
+    requires var byz := s.all_nodes - s.honest_nodes_states.Keys; |byz| < f(|s.all_nodes|)
+    requires forall m | 
+                                && m in s.att_network.messagesInTransit
+                            ::
+                                m.message in s.att_network.allMessagesSent;
+
+    // requires attestation_share in dvn.att_network.allMessagesSent
+    requires pred_rcvd_attestation_shares_is_in_all_messages_sent(s)    
+    ensures pred_4_1_b(s)
+    {
+        match event 
+        {
+            case HonestNodeTakingStep(node, nodeEvent, nodeOutputs) =>
+                var s_node := s.honest_nodes_states[node];
+                var s'_node := s'.honest_nodes_states[node];
+                match nodeEvent
+                {
+                    case ServeAttstationDuty(attestation_duty) => 
+                        // Proved
+                        lemma_pred_4_1_b_f_serve_attestation_duty(s.honest_nodes_states[node], attestation_duty, s'.honest_nodes_states[node]);
+                        lemma_pred_4_1_b_helper(s, event, s');
+                        assert pred_4_1_b(s');                    
+                    case AttConsensusDecided(id, decided_attestation_data) => 
+                        // Proved
+                        lemma_pred_4_1_b_f_att_consensus_decided(s.honest_nodes_states[node], id, decided_attestation_data, s'.honest_nodes_states[node]);
+                        lemma_pred_4_1_b_helper(s, event, s');
+                        assert pred_4_1_b(s');                    
+                    case ReceviedAttesttionShare(attestation_share) => 
+                        assert multiset(addReceipientToMessages<AttestationShare>({attestation_share}, node)) <= s.att_network.messagesInTransit;
+
+                        assert MessaageWithRecipient(message := attestation_share, receipient := node) in s.att_network.messagesInTransit;        
+
+                        
+                        assert attestation_share in s.att_network.allMessagesSent;
+
+                        forall hn | hn in s.honest_nodes_states.Keys
+                        ensures forall a | 
+                                         a in s'.honest_nodes_states[hn].bn.attestations_submitted
+                                ::
+                                 exists hn', att_share: AttestationShare, fork_version :: pred_4_1_b_exists(s', hn', att_share, fork_version, a);            
+                        {
+                            if hn != node 
+                            {
+                                assert s'.honest_nodes_states[hn] == s.honest_nodes_states[hn];
+                                forall a | 
+                                         a in s'.honest_nodes_states[hn].bn.attestations_submitted
+                                ensures exists hn', att_share: AttestationShare, fork_version :: pred_4_1_b_exists(s', hn', att_share, fork_version, a);            
+                                {
+                                    assert a in s.honest_nodes_states[hn].bn.attestations_submitted;
+                                    var hn', att_share: AttestationShare, fork_version :| pred_4_1_b_exists(s, hn', att_share, fork_version, a);                                    
+                                    
+                                    assert pred_4_1_b_exists(s', hn', att_share, fork_version, a);
+
+                                    assert exists hn', att_share: AttestationShare, fork_version :: pred_4_1_b_exists(s', hn', att_share, fork_version, a);                                    
+                                }
+                            }
+                            else 
+                            {
+                                lemma_pred_4_1_b_f_listen_for_attestation_shares(
+                                    s_node,
+                                    attestation_share,
+                                    s'_node,
+                                    s
+                                );
+
+                                forall a | 
+                                         a in s'.honest_nodes_states[hn].bn.attestations_submitted
+                                ensures exists hn', att_share: AttestationShare, fork_version :: pred_4_1_b_exists(s', hn', att_share, fork_version, a);            
+                                {
+                                    // assert a in s.honest_nodes_states[hn].bn.attestations_submitted;
+                                    var hn', att_share: AttestationShare, fork_version :| pred_4_1_b_exists(s, hn', att_share, fork_version, a);                                    
+                                    
+                                    assert pred_4_1_b_exists(s', hn', att_share, fork_version, a);
+
+                                    assert exists hn', att_share: AttestationShare, fork_version :: pred_4_1_b_exists(s', hn', att_share, fork_version, a);                                    
+                                }                                
+
+                                // assert forall a | a in s'_node.bn.attestations_submitted :: exists hn', att_share: AttestationShare, fork_version :: pred_4_1_b_exists(s', hn', att_share, fork_version, a);                                
+                            }
+                        }
+
+                        assert pred_4_1_b(s');         
+
+                    case ImportedNewBlock(block) => 
+                        // Provded
+                        var s_node := add_block_to_bn(s_node, nodeEvent.block);
+                        lemma_pred_4_1_b_f_listen_for_new_imported_blocks(s_node, block, s'_node);
+                        lemma_pred_4_1_b_helper(s, event, s');
+                        assert pred_4_1_b(s');                    
+                    case ResendAttestationShares => 
+                        // Proved
+                        lemma_pred_4_1_b_helper(s, event, s');
+                        assert pred_4_1_b(s');                    
+                    case NoEvent => 
+                        // Proved
+                        lemma_pred_4_1_b_helper(s, event, s');
+                        assert pred_4_1_b(s');
+                }
+
+            case AdeversaryTakingStep(node, new_attestation_share_sent, messagesReceivedByTheNode) =>
+                lemma_pred_4_1_b_helper(s, event, s');
+                assert pred_4_1_b(s');
+        }
+    }    
+
+    lemma lemma_pred_rcvd_attestation_shares_is_in_all_messages_sent(
+        s: DVState,
+        event: DV.Event,
+        s': DVState
+    )
+    requires NextEvent(s, event, s')
+    requires pred_rcvd_attestation_shares_is_in_all_messages_sent(s)
+    {
+        match event 
+        {
+            case HonestNodeTakingStep(node, nodeEvent, nodeOutputs) =>
+                var s_node := s.honest_nodes_states[node];
+                var s'_node := s'.honest_nodes_states[node];
+                match nodeEvent
+                {
+                    case ServeAttstationDuty(attestation_duty) => 
+                        // assert pred_rcvd_attestation_shares_is_in_all_messages_sent(s');                    
+                    case AttConsensusDecided(id, decided_attestation_data) => 
+                        // assert pred_rcvd_attestation_shares_is_in_all_messages_sent(s');                    
+                    case ReceviedAttesttionShare(attestation_share) => 
+                        // assert pred_rcvd_attestation_shares_is_in_all_messages_sent(s');
+
+                    case ImportedNewBlock(block) => 
+                        // assert pred_rcvd_attestation_shares_is_in_all_messages_sent(s');                    
+                    case ResendAttestationShares => 
+                        assert pred_rcvd_attestation_shares_is_in_all_messages_sent(s');                    
+                    case NoEvent => 
+                        assert pred_rcvd_attestation_shares_is_in_all_messages_sent(s');
+                }
+
+            case AdeversaryTakingStep(node, new_attestation_share_sent, messagesReceivedByTheNode) =>
+                assert pred_rcvd_attestation_shares_is_in_all_messages_sent(s');
+        }
+    }        
 }
